src/Pipit.Exp.Base.fst
@@ -1,3 +1,4 @@
+(* Definition of base expression type *)
 module Pipit.Exp.Base
 module C = Pipit.Context
 open Pipit.Inhabited
@@ -38,102 +39,11 @@ type exp (c: C.context) 'a =
   // check "" e in e
   | XCheck : string -> exp c xprop -> exp c 'a -> exp c 'a
 
-let rec open1' (#c: C.context) (e: exp c 'a) (n: C.index { C.has_index c n }) (x: C.var (C.get_index c n)): Tot (exp (C.open1' c n) 'a) (decreases e) =
-  match e with
-  | XVal v -> XVal v
-  | XBVar i ->
-    if i = n
-    then
-      XVar x
-    else
-      (C.open_preserves_opt_index_lemma c n i;
-      XBVar (C.index_drop i n 1))
-  | XVar x' ->
-    XVar x'
-  | XApp f e -> XApp (open1' f n x) (open1' e n x)
-  | XFby v e -> XFby v (open1' e n x)
-  | XThen e1 e2 -> XThen (open1' e1 n x) (open1' e2 n x)
-  | XMu _ e -> XMu (open1' e (n + 1) x)
-  | XLet b e1 e2 ->
-    let e1' = open1' e1 n x in
-    let e2' = open1' e2 (n + 1) x in
-    XLet b e1' e2'
-  | XCheck name e1 e2 -> XCheck name (open1' e1 n x) (open1' e2 n x)
-
-let rec close1' (#c: C.context) (e: exp c 'a) (x: C.var 'b) (n: C.index { n <= List.Tot.length c }): Tot (exp (C.close1' c 'b n) 'a) (decreases e) =
-  match e with
-  | XVal v -> XVal v
-  | XBVar i ->
-    C.close_preserves_opt_index_lemma c 'b n i;
-    XBVar (C.index_lift i n 1)
-  | XVar x' ->
-    if C.var_eq x x'
-    then
-      (C.close_contains_lemma c 'b n;
-      XBVar n)
-    else
-      (// C.close_preserves_opt_var_lemma c x n x';
-      XVar x')
-  | XApp f e -> XApp (close1' f x n) (close1' e x n)
-  | XFby v e -> XFby v (close1' e x n)
-  | XThen e1 e2 -> XThen (close1' e1 x n) (close1' e2 x n)
-  | XMu _ e -> XMu (close1' e x (n + 1))
-  | XLet b e1 e2 -> XLet b (close1' e1 x n) (close1' e2 x (n + 1))
-  | XCheck name e1 e2 -> XCheck name (close1' e1 x n) (close1' e2 x n)
-
-let open1 (e: exp 'c 'a { C.has_index 'c 0 }) x = open1' e 0 x
-let close1 (e: exp 'c 'a) x = close1' e x 0
-
-let rec lift1' (#c: C.context) (e: exp c 'a) (n: C.index { n <= List.Tot.length c }) (t: Type): Tot (exp (C.lift1 c n t) 'a) (decreases e) =
-  match e with
-  | XVal v -> XVal v
-  | XBVar i ->
-    // C.bind_index_preserves_opt_index_lemma c n i t;
-    C.close_preserves_opt_index_lemma c t n i;
-    XBVar (C.index_lift i n 1)
-  | XVar x' ->
-    XVar x'
-  | XApp f e -> XApp (lift1' f n t) (lift1' e n t)
-  | XFby v e -> XFby v (lift1' e n t)
-  | XThen e1 e2 -> XThen (lift1' e1 n t) (lift1' e2 n t)
-  | XMu _ e1 ->
-    let e1': exp (C.lift1 (C.lift1 c 0 'a) (n + 1) t) 'a = lift1' e1 (n + 1) t in
-    let e1'': exp (C.lift1 (C.lift1 c n t) 0 'a) 'a = e1' in
-    XMu e1''
-  | XLet b e1 e2 -> XLet b (lift1' e1 n t) (lift1' e2 (n + 1) t)
-  | XCheck name e1 e2 -> XCheck name (lift1' e1 n t) (lift1' e2 n t)
-
-let lift1 (#c: C.context) (e: exp c 'a) (t: Type): exp (C.lift1 c 0 t) 'a =
-  lift1' e 0 t
-
-let rec subst_index1' (#c: C.context) (e: exp c 'a) (i: C.index { C.has_index c i }) (payload: exp (C.drop1 c i) (C.get_index c i)): Tot (exp (C.drop1 c i) 'a) (decreases e) =
-  match e with
-  | XVal v -> XVal v
-  | XBVar i' ->
-    if i' = i
-    then payload
-    else
-      (C.open_preserves_opt_index_lemma c i i';
-      XBVar (C.index_drop i' i 1))
-  | XVar x' -> XVar x'
-  | XApp f e -> XApp (subst_index1' f i payload) (subst_index1' e i payload)
-  | XFby v e -> XFby v (subst_index1' e i payload)
-  | XThen e1 e2 -> XThen (subst_index1' e1 i payload) (subst_index1' e2 i payload)
-  | XMu _ e1 ->
-    let e1': exp (C.drop1 (C.lift1 c 0 'a) (i + 1)) 'a = subst_index1' e1 (i + 1) (lift1 payload 'a) in
-    let e1'': exp (C.lift1 (C.drop1 c i) 0 'a) 'a = e1' in
-    XMu e1''
-  | XLet b e1 e2 -> XLet b (subst_index1' e1 i payload) (subst_index1' e2 (i + 1) (lift1 payload b))
-  | XCheck name e1 e2 -> XCheck name (subst_index1' e1 i payload) (subst_index1' e2 i payload)
-
-let subst_index1 (#c: C.context { C.has_index c 0 }) (e: exp c 'a) (payload: exp (C.drop1 c 0) (C.get_index c 0)): Tot (exp (C.drop1 c 0) 'a) (decreases e) =
-  subst_index1' e 0 payload
-
 let rec weaken (#c c': C.context) (e: exp c 'a): Tot (exp (C.append c c') 'a) (decreases e) =
   match e with
   | XVal v -> XVal v
   | XBVar i' ->
-    C.append_preserves_opt_index_lemma c c' i';
+    C.lemma_append_preserves_opt_index c c' i';
     XBVar i'
   | XVar x' -> XVar x'
   | XApp f e -> XApp (weaken c' f) (weaken c' e)
