src/Pipit.Exp.Binding.fst
@@ -1,0 +1,243 @@
+(* Manipulating bindings: opening, closing, substituting and lifting *)
+module Pipit.Exp.Binding
+
+open Pipit.Exp.Base
+module C = Pipit.Context
+
+(* Open an expression so that a bound variable becomes free.
+   Not currently used. *)
+let rec open1' (#c: C.context) (e: exp c 'a) (n: C.index { C.has_index c n }) (x: C.var (C.get_index c n)): Tot (exp (C.open1' c n) 'a) (decreases e) =
+  match e with
+  | XVal v -> XVal v
+  | XBVar i ->
+    if i = n
+    then
+      XVar x
+    else
+      (C.lemma_open_preserves_opt_index c n i;
+      XBVar (C.index_drop i n 1))
+  | XVar x' ->
+    XVar x'
+  | XApp f e -> XApp (open1' f n x) (open1' e n x)
+  | XFby v e -> XFby v (open1' e n x)
+  | XThen e1 e2 -> XThen (open1' e1 n x) (open1' e2 n x)
+  | XMu _ e -> XMu (open1' e (n + 1) x)
+  | XLet b e1 e2 ->
+    let e1' = open1' e1 n x in
+    let e2' = open1' e2 (n + 1) x in
+    XLet b e1' e2'
+  | XCheck name e1 e2 -> XCheck name (open1' e1 n x) (open1' e2 n x)
+
+let open1 (e: exp 'c 'a { C.has_index 'c 0 }) x = open1' e 0 x
+
+(* Close an expression so that a free variable becomes bound.
+   This is used by the syntactic sugar, but not in the semantics. *)
+let rec close1' (#c: C.context) (e: exp c 'a) (x: C.var 'b) (n: C.index { n <= List.Tot.length c }): Tot (exp (C.close1' c 'b n) 'a) (decreases e) =
+  match e with
+  | XVal v -> XVal v
+  | XBVar i ->
+    C.lemma_close_preserves_opt_index c 'b n i;
+    XBVar (C.index_lift i n 1)
+  | XVar x' ->
+    if C.var_eq x x'
+    then
+      (C.lemma_close_contains c 'b n;
+      XBVar n)
+    else
+      XVar x'
+  | XApp f e -> XApp (close1' f x n) (close1' e x n)
+  | XFby v e -> XFby v (close1' e x n)
+  | XThen e1 e2 -> XThen (close1' e1 x n) (close1' e2 x n)
+  | XMu _ e -> XMu (close1' e x (n + 1))
+  | XLet b e1 e2 -> XLet b (close1' e1 x n) (close1' e2 x (n + 1))
+  | XCheck name e1 e2 -> XCheck name (close1' e1 x n) (close1' e2 x n)
+
+let close1 (e: exp 'c 'a) x = close1' e x 0
+
+(* Lift an expression by incrementing bound variable indices at or above n.
+   This is used directly by substitution, so we need to prove some properties
+   about it. Could we implement this in terms of close1' with a dummy free
+   variable? *)
+let rec lift1' (#c: C.context) (e: exp c 'a) (n: C.index { n <= List.Tot.length c }) (t: Type): Tot (exp (C.lift1 c n t) 'a) (decreases e) =
+  match e with
+  | XVal v -> XVal v
+  | XBVar i ->
+    C.lemma_close_preserves_opt_index c t n i;
+    XBVar (C.index_lift i n 1)
+  | XVar x' ->
+    XVar x'
+  | XApp f e -> XApp (lift1' f n t) (lift1' e n t)
+  | XFby v e -> XFby v (lift1' e n t)
+  | XThen e1 e2 -> XThen (lift1' e1 n t) (lift1' e2 n t)
+  | XMu _ e1 ->
+    let e1': exp (C.lift1 (C.lift1 c 0 'a) (n + 1) t) 'a = lift1' e1 (n + 1) t in
+    let e1'': exp (C.lift1 (C.lift1 c n t) 0 'a) 'a = e1' in
+    XMu e1''
+  | XLet b e1 e2 -> XLet b (lift1' e1 n t) (lift1' e2 (n + 1) t)
+  | XCheck name e1 e2 -> XCheck name (lift1' e1 n t) (lift1' e2 n t)
+
+let lift1 (#c: C.context) (e: exp c 'a) (t: Type): exp (C.lift1 c 0 t) 'a =
+  lift1' e 0 t
+
+(* Substitute one bound variable for a bound expression.
+   This is used by the semantics, so we need to prove that it commutes. *)
+let rec subst1' (#c: C.context) (e: exp c 'a) (i: C.index { C.has_index c i }) (payload: exp (C.drop1 c i) (C.get_index c i)): Tot (exp (C.drop1 c i) 'a) (decreases e) =
+  match e with
+  | XVal v -> XVal v
+  | XBVar i' ->
+    if i' = i
+    then payload
+    else
+      (C.lemma_open_preserves_opt_index c i i';
+      XBVar (C.index_drop i' i 1))
+  | XVar x' -> XVar x'
+  | XApp f e -> XApp (subst1' f i payload) (subst1' e i payload)
+  | XFby v e -> XFby v (subst1' e i payload)
+  | XThen e1 e2 -> XThen (subst1' e1 i payload) (subst1' e2 i payload)
+  | XMu _ e1 ->
+    let e1': exp (C.drop1 (C.lift1 c 0 'a) (i + 1)) 'a = subst1' e1 (i + 1) (lift1 payload 'a) in
+    let e1'': exp (C.lift1 (C.drop1 c i) 0 'a) 'a = e1' in
+    XMu e1''
+  | XLet b e1 e2 -> XLet b (subst1' e1 i payload) (subst1' e2 (i + 1) (lift1 payload b))
+  | XCheck name e1 e2 -> XCheck name (subst1' e1 i payload) (subst1' e2 i payload)
+
+let subst1 (#c: C.context { C.has_index c 0 }) (e: exp c 'a) (payload: exp (C.drop1 c 0) (C.get_index c 0)): Tot (exp (C.drop1 c 0) 'a) (decreases e) =
+  subst1' e 0 payload
+
+#push-options "--split_queries always"
+
+private
+let lemma_lift_lift_commute_XApp (e1: exp 'c ('b -> 'a)) (e2: exp 'c 'b) (i1: C.index { C.has_index 'c i1 }) (i2: C.index { i2 <= i1 }) (t1 t2: Type):
+  Lemma
+    (requires (lift1' (lift1' e1 i1 t1) i2 t2 === lift1' (lift1' e1 i2 t2) (i1 + 1) t1) /\
+              (lift1' (lift1' e2 i1 t1) i2 t2 === lift1' (lift1' e2 i2 t2) (i1 + 1) t1))
+    (ensures (lift1' (lift1' (XApp e1 e2) i1 t1) i2 t2 === lift1' (lift1' (XApp e1 e2) i2 t2) (i1 + 1) t1))
+     =
+  C.lemma_lift_lift_commute 'c i1 i2 t1 t2;
+  // calc (==) {
+  //  (lift1' (XApp e1 e2) i1 t1);
+  //  == { () }
+  //  XApp (lift1' e1 i1 t1) (lift1' e2 i1 t1);
+  // };
+ //  assert ((lift1' (XApp e1 e2) i1 t1) == XApp (lift1' e1 i1 t1) (lift1' e2 i1 t1)) by (FStar.Tactics.norm [delta; primops; iota; nbe; zeta]; FStar.Tactics.dump "ok");
+  assert_norm ((lift1' (XApp e1 e2) i1 t1) == XApp (lift1' e1 i1 t1) (lift1' e2 i1 t1));
+  assert_norm (lift1' (XApp (lift1' e1 i1 t1) (lift1' e2 i1 t1)) i2 t2 == XApp (lift1' (lift1' e1 i1 t1) i2 t2) (lift1' (lift1' e2 i1 t1) i2 t2) );
+  assert (XApp (lift1' (lift1' e1 i1 t1) i2 t2) (lift1' (lift1' e2 i1 t1) i2 t2) == XApp (lift1' (lift1' e1 i2 t2) (i1 + 1) t1) (lift1' (lift1' e2 i2 t2) (i1 + 1) t1));
+  assert_norm ((lift1' (lift1' (XApp e1 e2) i2 t2) (i1 + 1) t1) == XApp (lift1' (lift1' e1 i2 t2) (i1 + 1) t1) (lift1' (lift1' e2 i2 t2) (i1 + 1) t1));
+  // assert (
+  //   lift1' (lift1' (XApp e1 e2) i2 t2) (i1 + 1) t1) by (FStar.Tactics.norm [delta; primops; iota; nbe]; FStar.Tactics.dump "ok");
+  ()
+
+let rec lemma_lift_lift_commute (e: exp 'c 'a) (i1: C.index { C.has_index 'c i1 }) (i2: C.index { i2 <= i1 }) (t1 t2: Type):
+  Lemma (ensures (lift1' (lift1' e i1 t1) i2 t2 === lift1' (lift1' e i2 t2) (i1 + 1) t1))
+  // Lemma (ensures (C.lemma_lift_lift_commute 'c i1 i2 t1 t2;
+  //   lift1' (lift1' e i1 t1) i2 t2 == lift1' (lift1' e i2 t2) (i1 + 1) t1))
+    (decreases e) =
+  C.lemma_lift_lift_commute 'c i1 i2 t1 t2;
+  match e with
+  | XVal _ -> ()
+  | XBVar _ -> ()
+  | XVar _ -> ()
+  | XApp e1 e2 ->
+    lemma_lift_lift_commute e1 i1 i2 t1 t2;
+    lemma_lift_lift_commute e2 i1 i2 t1 t2;
+    lemma_lift_lift_commute_XApp e1 e2 i1 i2 t1 t2
+  | XFby v e1 ->
+    lemma_lift_lift_commute e1 i1 i2 t1 t2
+  | XThen e1 e2 ->
+    lemma_lift_lift_commute e1 i1 i2 t1 t2;
+    lemma_lift_lift_commute e2 i1 i2 t1 t2
+  | XMu _ e1 ->
+    lemma_lift_lift_commute e1 (i1 + 1) (i2 + 1) t1 t2
+  | XLet _ e1 e2 ->
+    lemma_lift_lift_commute e1 i1 i2 t1 t2;
+    lemma_lift_lift_commute e2 (i1 + 1) (i2 + 1) t1 t2
+  | XCheck _ e1 e2 ->
+    lemma_lift_lift_commute e1 i1 i2 t1 t2;
+    lemma_lift_lift_commute e2 i1 i2 t1 t2
+
+let rec subst_lift_id (e: exp 'c 'a) (i: C.index { C.has_index 'c i }) (p: exp 'c (C.get_index 'c i)) (t: Type):
+  Lemma (ensures subst1' (lift1' e i t) i p === e) =
+  C.lemma_drop_lift_eq 'c i t;
+  match e with
+  | XVal _ -> ()
+  | XVar _ -> ()
+  | _ -> admit ()
+  // | XPrim2 _ e1 e2 ->
+  //   subst_lift_id e1 p x;
+  //   subst_lift_id e2 p x
+  // | XIte ep e1 e2 ->
+  //   subst_lift_id ep p x;
+  //   subst_lift_id e1 p x;
+  //   subst_lift_id e2 p x
+  // | XFby _ e1 -> subst_lift_id e1 p x
+  // | XThen e1 e2 ->
+  //   subst_lift_id e1 p x;
+  //   subst_lift_id e2 p x
+  // | XMu e1 ->
+  //   subst_lift_id e1 (lift p 0) (x + 1)
+  // | XLet b e1 e2 ->
+  //   subst_lift_id e1 p x;
+  //   subst_lift_id e2 (lift p 0) (x + 1)
+
+(*
+let rec lift_subst_distribute_le (e p: exp) (x1: var) (x2: var { x2 <= x1 }):
+  Lemma (ensures lift (subst e x1 p) x2 == subst (lift e x2) (x1 + 1) (lift p x2)) =
+  match e with
+  | XVal _ -> ()
+  | XVar _ -> ()
+  | XPrim2 _ e1 e2 ->
+    lift_subst_distribute_le e1 p x1 x2;
+    lift_subst_distribute_le e2 p x1 x2
+  | XIte ep e1 e2 ->
+    lift_subst_distribute_le ep p x1 x2;
+    lift_subst_distribute_le e1 p x1 x2;
+    lift_subst_distribute_le e2 p x1 x2
+  | XPre e1 -> lift_subst_distribute_le e1 p x1 x2
+  | XThen e1 e2 ->
+    lift_subst_distribute_le e1 p x1 x2;
+    lift_subst_distribute_le e2 p x1 x2
+  | XMu e1 ->
+    lift_subst_distribute_le e1 (lift p 0) (x1 + 1) (x2 + 1);
+    lemma_lift_lift_commute p x2 0
+  | XLet e1 e2 ->
+    lift_subst_distribute_le e1 p x1 x2;
+    lift_subst_distribute_le e2 (lift p 0) (x1 + 1) (x2 + 1);
+    lemma_lift_lift_commute p x2 0
+
+let rec subst_subst_distribute_le (e p1 p2: exp) (x1: var) (x2: var { x1 <= x2 }):
+  Lemma (ensures subst (subst e x1 p1) x2 p2 ==
+                 subst (subst e (x2 + 1) (lift p2 x1)) x1 (subst p1 x2 p2)) =
+  match e with
+  | XVal _ -> ()
+  | XVar x' ->
+    if x' = x2 + 1
+    then subst_lift_id p2 (subst p1 x2 p2) x1
+  | XPrim2 _ e1 e2 ->
+    subst_subst_distribute_le e1 p1 p2 x1 x2;
+    subst_subst_distribute_le e2 p1 p2 x1 x2
+  | XIte ep e1 e2 ->
+    subst_subst_distribute_le ep p1 p2 x1 x2;
+    subst_subst_distribute_le e1 p1 p2 x1 x2;
+    subst_subst_distribute_le e2 p1 p2 x1 x2
+  | XPre e1 ->
+    subst_subst_distribute_le e1 p1 p2 x1 x2
+  | XThen e1 e2 ->
+    subst_subst_distribute_le e1 p1 p2 x1 x2;
+    subst_subst_distribute_le e2 p1 p2 x1 x2
+  | XMu e1 ->
+    subst_subst_distribute_le e1 (lift p1 0) (lift p2 0) (x1 + 1) (x2 + 1);
+    lemma_lift_lift_commute p2 x1 0;
+    lift_subst_distribute_le p1 p2 x2 0
+  | XLet e1 e2 ->
+    subst_subst_distribute_le e1 p1 p2 x1 x2;
+    subst_subst_distribute_le e2 (lift p1 0) (lift p2 0) (x1 + 1) (x2 + 1);
+    lemma_lift_lift_commute p2 x1 0;
+    lift_subst_distribute_le p1 p2 x2 0
+
+let subst_subst_distribute_XMu (e p: exp) (x: var):
+  Lemma (ensures subst (subst e 0 (XMu e)) x p ==
+                 subst (subst e (x + 1) (lift p 0)) 0 (XMu (subst e (x + 1) (lift p 0)))) =
+ subst_subst_distribute_le e (XMu e) p 0 x
+
+*)
